proof of the L4 to L4_2 instance. some admits remain.
L4 to L4_2 is de-bruijn to named conversion.
Perhaps eval does not syntactically commute with the translation; at least I couldn't prove it.
It certainly does that upto alpha equality.
Thus a proof that alpha equal values have same overvations was required.

coq-paramcoq is now needed. `opam install coq-paramcoq` should suffice.
See README.md (8.7 branch) for details.

theories/L4_deBruijn/L4_2_to_L4_5.v
@@ -198,8 +198,8 @@ Proof using.
   simpl. unfold isprogram, closed in *. rewrite L4_2_to_L4_5_fvars; tauto.
 Qed.
 
-Let eval42 := @polyEval.eval_n (Named.TermAbsImplUnstrict variables.NVar L4Opid).
-Let eval45 := @eval_n (Named.TermAbsImplUnstrict variables.NVar L4_5Opid).
+Definition eval42 := @polyEval.eval_n (Named.TermAbsImplUnstrict variables.NVar L4Opid).
+Definition eval45 := @eval_n (Named.TermAbsImplUnstrict variables.NVar L4_5Opid).
 
 
 (**  can be obtained for free using a parametricity plugin 
