theories/L4_deBruijn/expression.v
@@ -730,6 +730,7 @@ Lemma evals_n_monotone:
                       forall (m:nat), evals_n (n + m) es = Some fs.
 Admitted.
 
+
 (***
 Lemma eval_n_weaken:
   forall (n:nat),
@@ -1715,8 +1716,8 @@ Proof using.
   apply my_exp_wf_ind; intros; simpl in *; try lia.
 Qed.
 
-Close Scope Z_scope.
 
+Close Scope Z_scope.
 
 Definition fnames (e:efnlst) : list (Ast.name) :=
 map fst (efnlst_as_list e).
@@ -1781,3 +1782,199 @@ Function eval_ns (n:nat) (e:exp) {struct n}: option exp :=
                | Var_e e => None
              end
   end.
+
+Lemma eval_ns_Some_Succ:
+  forall e (n:nat) v, eval_ns n e = Some v -> n = (S (n - 1))%nat.
+Proof.
+  induction n; intros.
+  - simpl in H. discriminate.
+  - omega.
+Qed.
+
+
+(* similar to eval_n_monotone *)
+Lemma eval_ns_monotone:
+  forall (n:nat) e f, eval_ns n e = Some f ->
+                      forall (m:nat), eval_ns (n + m) e = Some f.
+Admitted.
+
+
+
+Require Import CpdtTactics.
+Lemma exps_as_list_from_list vs:
+  exps_from_list (exps_as_list vs) = vs.
+Proof using.
+  induction vs; crush.
+Qed.
+
+Require Import SquiggleEq.UsefulTypes.
+Require Import SquiggleEq.list.
+
+(* Move to SquiggleEq.list
+*)
+Lemma flattenLift {A B:Type} (f: A-> option B) g  l:
+  (forall b, isSome (f b) -> f b = g b)
+  -> (forall b, isSome (g b) -> isSome (f b))
+  -> flatten (map f l) = flatten (map g l).
+Proof using.
+  intros Heq Hn.
+  induction l;crush.
+  specialize (Heq a).
+  specialize (Hn a).
+  destruct (f a).
+- unfold isSome in Heq.
+  specialize (Heq (ltac:(auto))).
+  rewrite <- Heq. congruence.
+- clear Heq. destruct (g a); firstorder.
+Qed.
+
+(* Move to SquiggleEq.list
+*)
+Lemma flattenSomeCons {A:Type} (loa: list (option A)) a:
+  isSome (flatten (a::loa))
+  -> isSome (flatten loa).
+Proof using.
+  intros Hs.
+  simpl in Hs.
+  destruct a; firstorder.
+  destruct (flatten loa); firstorder.
+Qed.
+
+Require Import SquiggleEq.tactics.
+
+(* Move to SquiggleEq.list
+*)
+Lemma flattenSomeIn {A:Type} (loa: list (option A)) a:
+  isSome (flatten loa)
+  -> In a loa -> isSome a.
+Proof using.
+  revert a.
+  induction loa as [ | a loa]; destruct a; intros aa; destruct aa; try (crush; fail).
+  intros Hs Hin. apply False_ind.
+  apply flattenSomeCons in Hs.
+  dorn Hin; firstorder.
+  inversion Hin.
+Qed.  
+  
+
+(* Move to SquiggleEq.list
+*)
+Lemma flattenLift2 {A B:Type} (f: A-> option B) g  l:
+  (forall b, In b l -> f b = g b)
+  -> isSome (flatten (map f l))
+  -> flatten (map f l) = flatten (map g l).
+Proof using.
+  intros Heq Hs.
+  induction l; try (crush; fail).
+  pose proof Heq as Heqb.
+  specialize (Heq a). simpl.
+  pose proof Hs as Hsb.
+  simpl in Hsb.
+  destruct (f a);[ | firstorder].
+  specialize (Heq (ltac:(simpl;auto))).
+  rewrite <- Heq.
+  apply flattenSomeCons in Hs.
+  rewrite IHl;[reflexivity | firstorder| assumption].
+Qed.
+
+(* Move to SquiggleEq.Usefultypes
+*)
+Lemma isSomeIf {A:Type} oa (a: A):
+  oa = Some a -> isSome oa.
+Proof using.
+  crush.
+Qed.
+
+(** [eval_n] is complete w.r.t. [eval] **)
+Lemma eval_evalns:
+  (forall (e v:exp), eval e v -> exists (n:nat), eval_ns n e = Some v) /\
+  (forall (es vs:exps), evals es vs -> exists (n:nat), flatten (map (eval_ns n) (exps_as_list es))
+                                          = Some (exps_as_list vs)).
+Proof.
+  apply my_eval_ind; intros; try (solve [exists 1%nat; reflexivity]).
+  (* prove that if eval_ns becomes Some _, then n>0, similar to eval_n_Some_Succ
+    then prove evan_ns_monotone*)
+  - destruct H as [x h]. destruct H0 as [x0 h0]. destruct H1 as [x1 h1].
+    exists (x+x0+x1)%nat. simpl in *.
+    assert (j:=eval_ns_Some_Succ _ _ _ h).
+    assert (j0:=eval_ns_Some_Succ _ _ _ h0).
+    assert (j1:=eval_ns_Some_Succ _ _ _ h1).
+    assert (k:= eval_ns_monotone _ _ _ h).
+    assert (k0:= eval_ns_monotone _ _ _ h0).
+    assert (k1:= eval_ns_monotone _ _ _ h1).
+    rewrite j.
+    replace (S (x - 1) + x0 + x1)%nat
+    with (S (x + (x0 + x1 - 1)))%nat; try lia.
+    simpl. rewrite k.
+    replace (x + (x0 + x1 - 1))%nat with (x0 + (x + x1 - 1))%nat; try lia.
+    rewrite k0.
+    replace (x0 + (x + x1 - 1))%nat with (x1 + (x + x0 - 1))%nat; try lia.
+    rewrite k1. reflexivity.
+  - destruct H as [x h]. exists (x+1)%nat.
+    simpl. rewrite Nat.add_comm. simpl.
+    rewrite h. simpl.
+    rewrite exps_as_list_from_list. reflexivity.
+  - destruct H as [x h]. destruct H0 as [x0 h0].
+    assert (j:=eval_ns_Some_Succ _ _ _ h).
+    assert (j0:=eval_ns_Some_Succ _ _ _ h0).
+    assert (k:= eval_ns_monotone _ _ _ h).
+    assert (k0:= eval_ns_monotone _ _ _ h0).
+    exists (x+x0)%nat.
+    rewrite j.
+    replace (S (x - 1) + x0)%nat with (S (x + (x0 - 1)))%nat; try lia.
+    simpl. rewrite k.
+    replace (x + (x0 - 1))%nat with (x0 + (x - 1))%nat; try lia.
+    rewrite k0. reflexivity.
+  - destruct H as [x h]. destruct H0 as [x0 h0].
+    assert (j:=eval_ns_Some_Succ _ _ _ h).
+    assert (j0:=eval_ns_Some_Succ _ _ _ h0).
+    assert (k:= eval_ns_monotone _ _ _ h).
+    assert (k0:= eval_ns_monotone _ _ _ h0).
+    exists (x+x0)%nat.
+    rewrite j.
+    replace (S (x - 1) + x0)%nat with (S (x + (x0 - 1)))%nat; try lia.
+    simpl. rewrite k. subst vs'.
+    replace (x + (x0 - 1))%nat with (x0 + (x - 1))%nat; try lia.
+    replace (exps_skipn p vs) with vs in e1, k0 by admit. (* fix eval *)
+    rewrite e1. rewrite k0. reflexivity.
+  - destruct H as [x h]. destruct H0 as [x0 h0]. destruct H1 as [x1 h1].
+    exists (x+x0+x1)%nat.
+    assert (j:=eval_ns_Some_Succ _ _ _ h).
+    assert (j0:=eval_ns_Some_Succ _ _ _ h0).
+    assert (j1:=eval_ns_Some_Succ _ _ _ h1).
+    assert (k:= eval_ns_monotone _ _ _ h).
+    assert (k0:= eval_ns_monotone _ _ _ h0).
+    assert (k1:= eval_ns_monotone _ _ _ h1).
+    rewrite j.
+    replace (S (x - 1) + x0 + x1)%nat
+    with (S (x + (x0 + x1 - 1)))%nat; try lia.
+    simpl. rewrite k.
+    replace (x + (x0 + x1 - 1))%nat with (x0 + (x + x1 - 1))%nat; try lia.
+    rewrite k0.
+    replace (x0 + (x + x1 - 1))%nat with (x1 + (x + x0 - 1))%nat; try lia.
+    rewrite e3, k1. reflexivity.
+  - destruct H as [x h].
+    destruct H0 as [x0 h0].
+    assert (j:=eval_ns_Some_Succ _ _ _ h).
+    assert (j0:=eval_ns_Some_Succ _ _ _ h0).
+    assert (k:= eval_ns_monotone _ _ _ h).
+    assert (k0:= eval_ns_monotone _ _ _ h0).
+    exists (S (x+x0)%nat). simpl. rewrite k.
+    rewrite Nat.add_comm. rewrite k0. reflexivity.
+  - simpl. exrepnd. exists (n0+n)%nat.
+    assert (k:= eval_ns_monotone _ _ _ H0). clear H0.
+    rewrite k.
+    erewrite <- flattenLift2;[ | | rewrite H1; firstorder];[rewrite H1; refl | ].
+    intros.
+    apply in_map with (f:= (eval_ns n))in H.
+    apply isSomeIf in H1.
+    eapply flattenSomeIn in H1; eauto.
+    remember (eval_ns n b) as r.
+    destruct r; [ | firstorder].
+    symmetry.
+    rewrite Nat.add_comm.
+    apply  eval_ns_monotone.
+    auto.
+
+    Fail idtac. (* done except for the admit above *)
+Admitted.
